scheduler/SchIAproof.v
@@ -2,7 +2,7 @@ Require Import CRIS.
 
 Require Import SchGInv SchHeader SchI SchA.
 
-Require Import wpsim.
+Require Import wpsim_tactics ltac2_lib.
 
 Set Implicit Arguments.
 
@@ -159,268 +159,6 @@ Module SchIA. Section SchIA.
   Local Notation SchAMod := (SchA.t υ n Spc_global Spc_user).
   Local Notation SchIMod := (SchI.t).
 
-From iris.proofmode Require Import coq_tactics environments.
-(* ● ◓ ○ *)
-Notation "E1 '------------------------------------------------------------------□' E2 '------------------------------------------------------------------∗' st_src st_tgt '------------------------------params------------------------------' ○ n E r g ps pt '-------------------------------wsim-------------------------------' itr_src itr_tgt" :=
-  (environments.envs_entails (Envs E1 E2 _) (wpsim _ _ _ _ None _ _ n E r g _ _ _ ps pt _ (st_src, itr_src) (st_tgt, itr_tgt)))
-    (at level 50, only printing,
-      format "E1 '------------------------------------------------------------------□' '//' E2 '------------------------------------------------------------------∗' '//' st_src '//' st_tgt '//' '------------------------------params------------------------------' '//' ○ '/' n '/' E '/' r '/' g '/' ps '/' pt '//' '-------------------------------wsim-------------------------------' '//' itr_src '//' '//' '//' itr_tgt '//'").
-Notation "E1 '------------------------------------------------------------------□' E2 '------------------------------------------------------------------∗' st_src st_tgt '------------------------------params------------------------------' ◓ n E r g ps pt '-------------------------------wsim-------------------------------' itr_src itr_tgt" :=
-  (environments.envs_entails (Envs E1 E2 _) (wpsim _ _ _ _ (Some false) _ _ n E r g _ _ _ ps pt _ (st_src, itr_src) (st_tgt, itr_tgt)))
-    (at level 50, only printing,
-      format "E1 '------------------------------------------------------------------□' '//' E2 '------------------------------------------------------------------∗' '//' st_src '//' st_tgt '//' '------------------------------params------------------------------' '//' ◓ '/' n '/' E '/' r '/' g '/' ps '/' pt '//' '-------------------------------wsim-------------------------------' '//' itr_src '//' '//' '//' itr_tgt '//'").
-Notation "E1 '------------------------------------------------------------------□' E2 '------------------------------------------------------------------∗' st_src st_tgt '------------------------------params------------------------------' ● n E r g ps pt '-------------------------------wsim-------------------------------' itr_src itr_tgt" :=
-  (environments.envs_entails (Envs E1 E2 _) (wpsim _ _ _ _ (Some true) _ _ n E r g _ _ _ ps pt _ (st_src, itr_src) (st_tgt, itr_tgt)))
-    (at level 50, only printing,
-      format "E1 '------------------------------------------------------------------□' '//' E2 '------------------------------------------------------------------∗' '//' st_src '//' st_tgt '//' '------------------------------params------------------------------' '//' ● '/' n '/' E '/' r '/' g '/' ps '/' pt '//' '-------------------------------wsim-------------------------------' '//' itr_src '//' '//' '//' itr_tgt '//'").
-Notation "E1 '------------------------------------------------------------------□' st_src st_tgt '------------------------------params------------------------------' ○ n E r g ps pt '-------------------------------wsim-------------------------------' itr_src itr_tgt" :=
-  (environments.envs_entails (Envs E1 Enil _) (wpsim _ _ _ _ None _ _ n E r g _ _ _ ps pt _ (st_src, itr_src) (st_tgt, itr_tgt)))
-    (at level 50, only printing,
-      format "E1 '------------------------------------------------------------------□' '//' st_src '//' st_tgt '//' '------------------------------params------------------------------' '//' ○ '/' n '/' E '/' r '/' g '/' ps '/' pt '//' '-------------------------------wsim-------------------------------' '//' itr_src '//' '//' '//' itr_tgt '//'").
-Notation "E1 '------------------------------------------------------------------□' st_src st_tgt '------------------------------params------------------------------' ◓ n E r g ps pt '-------------------------------wsim-------------------------------' itr_src itr_tgt" :=
-  (environments.envs_entails (Envs E1 Enil _) (wpsim _ _ _ _ (Some false) _ _ n E r g _ _ _ ps pt _ (st_src, itr_src) (st_tgt, itr_tgt)))
-    (at level 50, only printing,
-      format "E1 '------------------------------------------------------------------□' '//' st_src '//' st_tgt '//' '------------------------------params------------------------------' '//' ◓ '/' n '/' E '/' r '/' g '/' ps '/' pt '//' '-------------------------------wsim-------------------------------' '//' itr_src '//' '//' '//' itr_tgt '//'").
-Notation "E1 '------------------------------------------------------------------□' st_src st_tgt '------------------------------params------------------------------' ● n E r g ps pt '-------------------------------wsim-------------------------------' itr_src itr_tgt" :=
-  (environments.envs_entails (Envs E1 Enil _) (wpsim _ _ _ _ (Some true) _ _ n E r g _ _ _ ps pt _ (st_src, itr_src) (st_tgt, itr_tgt)))
-    (at level 50, only printing,
-      format "E1 '------------------------------------------------------------------□' '//' st_src '//' st_tgt '//' '------------------------------params------------------------------' '//' ● '/' n '/' E '/' r '/' g '/' ps '/' pt '//' '-------------------------------wsim-------------------------------' '//' itr_src '//' '//' '//' itr_tgt '//'").
-Notation "E2 '------------------------------------------------------------------∗' st_src st_tgt '------------------------------params------------------------------' ○ n E r g ps pt '-------------------------------wsim-------------------------------' itr_src itr_tgt" :=
-  (environments.envs_entails (Envs Enil E2 _) (wpsim _ _ _ _ None _ _ n E r g _ _ _ ps pt _ (st_src, itr_src) (st_tgt, itr_tgt)))
-    (at level 50, only printing,
-      format "E2 '------------------------------------------------------------------∗' '//' st_src '//' st_tgt '//' '------------------------------params------------------------------' '//' ○ '/' n '/' E '/' r '/' g '/' ps '/' pt '//' '-------------------------------wsim-------------------------------' '//' itr_src '//' '//' '//' itr_tgt '//'").
-Notation "E2 '------------------------------------------------------------------∗' st_src st_tgt '------------------------------params------------------------------' ◓ n E r g ps pt '-------------------------------wsim-------------------------------' itr_src itr_tgt" :=
-  (environments.envs_entails (Envs Enil E2 _) (wpsim _ _ _ _ (Some false) _ _ n E r g _ _ _ ps pt _ (st_src, itr_src) (st_tgt, itr_tgt)))
-    (at level 50, only printing,
-      format "E2 '------------------------------------------------------------------∗' '//' st_src '//' st_tgt '//' '------------------------------params------------------------------' '//' ◓ '/' n '/' E '/' r '/' g '/' ps '/' pt '//' '-------------------------------wsim-------------------------------' '//' itr_src '//' '//' '//' itr_tgt '//'").
-Notation "E2 '------------------------------------------------------------------∗' st_src st_tgt '------------------------------params------------------------------' ● n E r g ps pt '-------------------------------wsim-------------------------------' itr_src itr_tgt" :=
-  (environments.envs_entails (Envs Enil E2 _) (wpsim _ _ _ _ (Some true) _ _ n E r g _ _ _ ps pt _ (st_src, itr_src) (st_tgt, itr_tgt)))
-    (at level 50, only printing,
-      format "E2 '------------------------------------------------------------------∗' '//' st_src '//' st_tgt '//' '------------------------------params------------------------------' '//' ● '/' n '/' E '/' r '/' g '/' ps '/' pt '//' '-------------------------------wsim-------------------------------' '//' itr_src '//' '//' '//' itr_tgt '//'").
-
-(* additional *) 
-(* Notation "E1 '------------------------------------------------------------------□' E2 '------------------------------------------------------------------∗' st_src st_tgt '-------------------------------wsim-------------------------------' P '∗' 'ISIM'" :=
-  (environments.envs_entails (Envs E1 E2 _) (bi_sep P (isim _ _ _ _ _ _ _ _ _ _ _ (st_src, _) (st_tgt, _))))
-    (at level 50, only printing,
-      format "E1 '------------------------------------------------------------------□' '//' E2 '------------------------------------------------------------------∗' '//' st_src '//' st_tgt '//' '-------------------------------wsim-------------------------------' '//' P  '∗'  'ISIM' ").
-
-Notation "E1 '------------------------------------------------------------------□' E2 '------------------------------------------------------------------∗' st_src st_tgt '-------------------------------wsim-------------------------------' P '-∗' 'ISIM'" :=
-  (environments.envs_entails (Envs E1 E2 _) (bi_wand P (isim _ _ _ _ _ _ _ _ _ _ _ (st_src, _) (st_tgt, _))))
-    (at level 50, only printing,
-      format "E1 '------------------------------------------------------------------□' '//' E2 '------------------------------------------------------------------∗' '//' st_src '//' st_tgt '//' '-------------------------------wsim-------------------------------' '//' P  '-∗'  'ISIM' "). *)
-
-  Ltac _w_step :=
-    match goal with
-    | [ |- environments.envs_entails _ (wpsim _ _ _ _ _ _ _ _ _ _ _ _ _ _ _ _ _ (_, Ret _) (_, Ret _))] =>
-        iApply wpsim_ret
-    | [ |- environments.envs_entails _ (wpsim _ _ _ _ _ _ _ _ _ _ _ _ _ _ _ _ _ (_, trigger (IO _ _) >>= _) (_, trigger (IO _ _) >>= _))] =>
-        iApply wpsim_io; iIntros "%"
-    | [ |- environments.envs_entails _ (wpsim _ _ _ _ _ _ _ _ _ _ _ _ _ _ _ _ _ (_, trigger (Spawn _ _) >>= _) (_, trigger (Spawn _ _) >>= _))] =>
-        iApply wpsim_spawn
-    end.
-
-  Ltac _w_step_l :=
-    match goal with
-    | [ |- environments.envs_entails _ (wpsim _ _ _ _ _ _ _ _ _ _ _ _ _ _ _ _ _ (_, tau;; _) _) ] =>
-        iApply wpsim_tau_src
-    | [ |- environments.envs_entails _ (wpsim _ _ _ _ _ _ _ _ _ _ _ _ _ _ _ _ _ (_, Ret _ >>= _) _) ] =>
-        rewrite bind_ret_l
-    | [ |- environments.envs_entails _ (wpsim _ _ _ _ _ _ _ _ _ _ _ _ _ _ _ _ _ (_, trigger Tid >>= _) _) ] =>
-        iApply wpsim_tid_src
-    | [ |- environments.envs_entails _ (wpsim _ _ _ _ _ _ _ _ _ _ _ _ _ _ _ _ _ (_, trigger (Take _) >>= _) _) ] =>
-        let name := fresh "q" in iApply wpsim_take_src; iIntros (name)
-    | [ |- environments.envs_entails _ (wpsim _ _ _ _ _ _ _ _ _ _ _ _ _ _ _ _ _ (_, trigger (Assume ?P) >>= _) _) ] =>
-        unfold_precond_postcond P; iApply wpsim_assume_src; iIntrosFresh "ASM"
-    | [ |- environments.envs_entails _ (wpsim _ _ _ _ _ _ _ _ _ _ _ _ _ _ _ _ _ (_, assume _ >>= _) _) ] =>
-        let name := fresh "asm" in iApply wpsim_asm_src; iIntros (name)
-    | [ |- environments.envs_entails _ (wpsim _ _ _ _ _ _ _ _ _ _ _ _ _ _ _ _ _ (_, (HModSem.sandbox _ (trigger (SPut _ _))) >>= _) _) ] =>
-        iApply wpsim_sput_src_sandbox; [s;eauto|]
-    | [ |- environments.envs_entails _ (wpsim _ _ _ _ _ _ _ _ _ _ _ _ _ _ _ _ _ (_, (HModSem.sandbox _ (trigger (SGet _))) >>= _) _) ] =>
-        iApply wpsim_sget_src_sandbox; [s;eauto|]
-    end.
-    (* 
-    | [ |- environments.envs_entails _ (isim _ _ _ _ _ _ _ _ _ _ _ (_, unwrapU ?ox >>= _) _) ] =>
-        let name := fresh "q" in
-        iApply isim_unwrapU_src; iIntros (name) "%";
-        match goal with [ H: ?x = Some _ |- _ ] => let G := fresh "G" in rename H into G; try rewrite -> G in * end
-    end. *)
-
-  Ltac _w_step_r :=
-    match goal with
-    (******* isim ******)
-    (** tgt **)
-    | [ |- environments.envs_entails _ (wpsim _ _ _ _ _ _ _ _ _ _ _ _ _ _ _ _ _ _ (_, tau;; _)) ] =>
-        iApply wpsim_tau_tgt
-    | [ |- environments.envs_entails _ (wpsim _ _ _ _ _ _ _ _ _ _ _ _ _ _ _ _ _ _ (_, Ret _ >>= _) ) ] =>
-        rewrite bind_ret_l
-    | [ |- environments.envs_entails _ (wpsim _ _ _ _ _ _ _ _ _ _ _ _ _ _ _ _ _ _ (_, trigger (Choose _) >>= _) ) ] =>
-        let name := fresh "q" in iApply wpsim_choose_tgt; iIntros (name)
-    | [ |- environments.envs_entails _ (wpsim _ _ _ _ _ _ _ _ _ _ _ _ _ _ _ _ _ _ (_, trigger (Guarantee ?P) >>= _) ) ] =>
-        unfold_precond_postcond P; iApply wpsim_guarantee_tgt; iIntrosFresh "GRT"
-    | [ |- environments.envs_entails _ (wpsim _ _ _ _ _ _ _ _ _ _ _ _ _ _ _ _ _ _ (_, guarantee _ >>= _)) ] =>
-        let name := fresh "grt" in iApply wpsim_guar_tgt; iIntros (name)
-    | [ |- environments.envs_entails _ (wpsim _ _ _ _ _ _ _ _ _ _ _ _ _ _ _ _ _ _ (_, (HModSem.sandbox _ (trigger (SPut _ _))) >>= _)) ] =>
-        iApply wpsim_sput_tgt_sandbox; [s; eauto|]
-    | [ |- environments.envs_entails _ (wpsim _ _ _ _ _ _ _ _ _ _ _ _ _ _ _ _ _ _ (_, (HModSem.sandbox _ (trigger (SGet _))) >>= _)) ] =>
-        iApply wpsim_sget_tgt_sandbox; [s; eauto|]
-    (* 
-    | [ |- environments.envs_entails _ (isim _ _ _ _ _ _ _ _ _ _ _ _ (_, unwrapN ?ox >>= _)) ] =>
-        let name := fresh "q" in
-        iApply isim_unwrapN_tgt; iIntros (name) "%";
-        match goal with [ H: ?x = Some _ |- _ ] => let G := fresh "G" in rename H into G; try rewrite -> G in * end
- *)
-    | [ |- environments.envs_entails _ (wpsim _ _ _ _ _ _ _ _ _ _ _ _ _ _ _ _ _ _ (_, trigger Tid >>= _)) ] =>
-        iApply wpsim_tid_tgt
-    end.
-
-  Ltac w_step_l_core :=
-    _w_step_l; try alist_find_simpl; s; des_pairs; s.
-  Ltac w_step_r_core :=
-    _w_step_r; try alist_find_simpl; s; des_pairs; s.
-
-  Ltac _w_force_l :=
-    match goal with
-    | [ |- environments.envs_entails _ (wpsim _ _ _ _ _ _ _ _ _ _ _ _ _ _ _ _ _ (_, trigger (Choose ?T) >>= _) _) ] =>
-        iApply wpsim_choose_src
-    | [ |- environments.envs_entails _ (wpsim _ _ _ _ _ _ _ _ _ _ _ _ _ _ _ _ _ (_, trigger (Guarantee ?P) >>= _) _) ] =>
-        unfold_precond_postcond P;
-        match goal with
-        | [|- environments.envs_entails _ (wpsim _ _ _ _ _ _ _ _ _ _ _ _ _ _ _ _ _ (_, trigger (Guarantee ?P) >>= _) _)] =>
-          match P with
-          | (wpsim_ginv _ _ _)%I => iApply wpsim_full_guarantee_src; iSplitL ""; first iIntros "I"; iFrame
-          | _ => iApply wpsim_guarantee_src
-          end
-        end
-    | [ |- environments.envs_entails _ (wpsim _ _ _ _ _ _ _ _ _ _ _ _ _ _ _ _ _ (_, unwrapN _ >>= _) _) ] =>
-        iApply wpsim_unwrapN_src
-    (* | [ |- environments.envs_entails _ (isim _ _ _ _ _ _ _ _ _ _ _ (_, guarantee _ >>= _) _) ] =>
-        iApply isim_guar_src *)
-    end.
-
-  Ltac w_force_l_core :=
-    let marker := fresh "MARKER" in
-    set_marker marker;
-    hide_ihyps;
-    hide_itree_r;
-    prep;
-    _w_force_l;
-    show_until marker.
-
-  Tactic Notation "w_force_l" :=
-    w_force_l_core; try (iExists _).
-
-  Tactic Notation "w_force_l" uconstr(p) :=
-    w_force_l_core; iExists p.
-
-  Ltac w_step :=
-    let marker := fresh "MARKER" in
-    set_marker marker;
-    hide_ihyps;
-    hide_itree_r; prep; show_itree;
-    hide_itree_l; prep; show_itree;
-    _w_step;
-    show_until marker.
-
-  Ltac w_step_l :=
-    let marker := fresh "MARKER" in
-    set_marker marker;
-    hide_ihyps;
-    hide_itree_r;
-    prep;
-    w_step_l_core;
-    show_until marker.
-
-  Ltac w_steps_l :=
-    let marker := fresh "MARKER" in
-    set_marker marker;
-    hide_ihyps;
-    hide_itree_r;
-    (hrepeat do 1 (prep; w_step_l_core));
-    show_until marker.
-
-  Ltac w_step_r :=
-    let marker := fresh "MARKER" in
-    set_marker marker;
-    hide_ihyps;
-    hide_itree_l;
-    prep;
-    w_step_r_core;
-    show_until marker.
-
-  Ltac w_steps_r :=
-    let marker := fresh "MARKER" in
-    set_marker marker;
-    hide_ihyps;
-    hide_itree_l;
-    (hrepeat do 1 (prep; w_step_r_core));
-    show_until marker.
-
-  Ltac by_coind CIH :=
-    iApply wpsim_progress; iApply wpsim_base;
-    iSpecialize (CIH $! _);
-    (hrepeat do 1 first[instantiate (1:= (_,_))|instantiate (1:= existT _ _)]); s; grind;
-    iApply CIH.
-
-  Ltac w_call hyps :=
-    let marker := fresh "MARKER" in
-    set_marker marker;
-    hide_ihyps;
-    hide_itree_r; prep; show_itree;
-    hide_itree_l; prep; show_itree;
-    iApply wpsim_call;
-    show_until marker;
-    iSplitL hyps; [try done | iIntros "% % % % % %"; iIntrosFresh "IST"];
-    move_aux.
-
-  Ltac yield hyps :=
-    let marker := fresh "MARKER" in
-    set_marker marker;
-    hide_ihyps;
-    hide_itree_r; prep; show_itree;
-    hide_itree_l; prep; show_itree;
-    iApply wpsim_yield
-    ; show_until marker
-    ; iSplitL hyps; [try done | iIntros "% % % % %"; iIntrosFresh "IST"]
-    ; move_aux
-    .
-
-  Ltac init_simF :=
-    pre_simF;
-    alist_find_simpl;
-    let H := fresh "H" in intro H; inv H;
-    alist_find_simpl;
-    post_simF;
-    step_l.
-
-  Ltac init_wpsim :=
-    init_simF;
-    prep_l;
-    match goal with
-    | [ |- environments.envs_entails _ (isim _ _ _ _ _ _ _ _ _ _ _ (_, trigger (Take _) >>= _) _)] =>
-      let name := fresh "q" in let n := fresh "n" in iApply isim_take_src; iIntros (name);
-        prep; let varg := fresh "varg" in iApply isim_take_src; iIntros (varg);
-        prep;
-        match goal with
-        | [ |- environments.envs_entails _ (isim _ _ _ _ _ _ _ _ _ _ _  (_, trigger (Assume ?P) >>= _) _) ] =>
-          unfold_precond_postcond P; iApply isim_Assume_src; iIntros "[I ASM]";
-          iApply wpsim_init; iSplitR "I"; last iExact "I"
-        end
-    end.
-
-  Ltac unfold_iter_l :=
-    let marker := fresh "MARKER" in
-    set_marker marker;
-    hide_ihyps;
-    hide_itree_r; rewrite unfold_iter_eq; show_itree;
-    show_until marker.
-
-  Ltac unfold_iter_r :=
-    let marker := fresh "MARKER" in
-    set_marker marker;
-    hide_ihyps;
-    hide_itree_l; rewrite unfold_iter_eq; show_itree;
-    show_until marker.
-
   Lemma simF__spawn : HSim.sim_fun open SchAMod SchIMod Ist SchName._spawn.
   Proof.
     init_wpsim.
@@ -431,19 +169,17 @@ Notation "E1 '------------------------------------------------------------------
     w_step_l. hss.
 
     (* Process yield *)
-    w_step_r. prep_l. rewrite /sch_ginv. w_force_l.
+    w_step_r. w_force_l. iSplitL ""; first done.
+
     prep_r. yield "IST".
     w_step_l.
-    prep_l. iApply wpsim_full_assume_src; iSplitL ""; first rewrite /sch_ginv; iIntros "I"; iFrame.
-    { iAssert (emp)%I as "E"; first done; iApply "E". }
-    iClear "I".
-    do 2 w_step_l.
-    do 2 w_step_r.
+    w_step_l; iClear "ASM".
+    w_steps_l. w_steps_r.
 
     (* Call the spawnee *)
     prep. inv H. rename x into userfspec. w_force_l userfspec; iFrame.
-    iSplit; first (iPureIntro; easy).
-    w_step_l.
+    iSplit; first (iPureIntro; apply FunInSpc; done).
+    w_steps_l.
 
     (* Choose the metavariables *)
     do 2 w_force_l.
@@ -477,7 +213,7 @@ Notation "E1 '------------------------------------------------------------------
     w_steps_r. hss.
 
     remember ([(SchI.v_ths, ((alist_replace my_tid (Some sret) ths_tgt): thslist) ↑)]) as st_tgt1.
-    iAssert (Ist sk nths'0 st_s'0 st_tgt1) with "[token THB THW COND POST]" as "IST".
+    iAssert (Ist nths'0 st_s'0 st_tgt1) with "[token THB THW COND POST]" as "IST".
     { destruct (alist_find my_tid ths_tgt) eqn:LU; cycle 1; [|destruct o].
       { (* idle case - impossible *)
         dup SIM. specialize (SIM my_tid). rewrite LU in SIM. inv SIM.
@@ -557,19 +293,13 @@ Notation "E1 '------------------------------------------------------------------
     destruct a as [nths1 [st_src1 [st_tgt1 [NODS1 NODD1]]]]. s.
     iIntros "IST _ #CIH".
     unfold_iter_l. unfold_iter_r.
-    (* rewrite {2}(@unfold_iter_eq hmodE). rewrite {2}(@unfold_iter_eq pmodE). *)
 
     w_step_l. w_step_l.
     w_force_l tt. w_force_l (tt↑).
-    prep_l.
-    iApply wpsim_full_guarantee_src_WP.
-    iSplitL ""; ss.
+    w_force_l. iSplitL ""; first ss.
 
     w_call "IST".
-    w_step_l.
-    prep_l.
-    iApply wpsim_full_assume_src_WP; iIntros "Q".
-    w_steps_l. rewrite {2}/postcond; ss. iDestruct "Q" as "[-> ->]". hss.
+    w_steps_l. iDestruct "ASM" as "[-> ->]". hss.
     w_steps_l.
     w_steps_r. hss. w_steps_r.
     by_coind "CIH".
@@ -606,7 +336,7 @@ Notation "E1 '------------------------------------------------------------------
     w_force_l. iSplitL "PRE TKNH".
     { iIntros "W". rewrite /token_half. unseal "SchA". iFrame. iPureIntro. esplits; et. }
 
-    prep_l. iApply wpsim_full_guarantee_src; iSplitL ""; first rewrite /sch_ginv; iFrame; eauto.
+    w_force_l. iSplitL ""; first done. 
 
     (* build IST *)
     rewrite /alist_upd /_alist_upd /=.
@@ -627,19 +357,12 @@ Notation "E1 '------------------------------------------------------------------
           rewrite right_id. et.
     }
     yield "IST"; et.
-    w_step_l.
-    prep_l. iApply wpsim_full_assume_src; iSplitL ""; first rewrite /sch_ginv; iIntros "I"; iFrame.
-    { iAssert (emp)%I as "E"; first done; iApply "E". }
-    iClear "I".
 
-    w_step_l. w_step_l. w_step_l. w_step_l. w_step_l.
-    w_step_r. w_step_r. w_step_r.
+    w_steps_l. iClear "ASM".
+    w_steps_r.
     w_force_l (nths ↑).
-    prep_l. iApply wpsim_full_guarantee_src; iSplitL "TKNQ0"; iFrame; eauto.
-    { repeat (unfold postcond; s).
-      iIntros "$"; iExists nths; iSplit; first done.
-      iExists nths; iSplit; et.
-    }
+    w_force_l.
+    iSplitL "TKNQ0"; iFrame; eauto.
     w_step. iFrame; easy.
     Unshelve. exact 1%positive. (* TODO: Erase!*)
   Qed.
@@ -654,20 +377,16 @@ Notation "E1 '------------------------------------------------------------------
     w_step_r. hss. w_step_r.
     w_step_r. w_step_r. w_step_r. w_step_r. w_step_r. w_step_r. w_step_r.
     w_force_l q. w_step_l. w_step_l.
-    prep_l. rewrite /sch_ginv; w_force_l.
+    w_force_l. iSplitL ""; first done.
     
     yield "THB THW COND".
     { iExists _, _, _, _. iSplit; et. iFrame. }
 
-    w_step_l.
-    prep_l. iApply wpsim_full_assume_src; iSplitL ""; first (iIntros "I"; iFrame; instantiate (1:=True%I); easy).
-    iIntros "_".
+    w_steps_l. iClear "ASM".
 
-    w_step_l. w_step_l. w_step_l.
     w_force_l (tt↑).
-    prep_l. iApply wpsim_full_guarantee_src; iSplitL "".
-    { iIntros "I"; iFrame. unfold postcond; s; iSplit; easy. }
-    w_step_r. w_step_r.
+    w_force_l; iSplitL ""; first done.
+    w_steps_r.
     w_step. iFrame; easy.
     Unshelve. exact 1%positive.
   Qed.
@@ -720,9 +439,7 @@ Notation "E1 '------------------------------------------------------------------
           rewrite -H4. iApply "POST".
         }
         
-        w_force_l. 
-        prep_l; iApply wpsim_full_guarantee_src; iSplitL "POST"; iFrame; et.
-        { rewrite /postcond /=; iIntros "$"; rewrite /postcond /=; iFrame; iSplit; easy. }
+        w_force_l. w_force_l. iSplitL "POST"; iFrame; et.
         assert (◯ (ths_src_w ⋅ (λ n: nat, if tid =? n then Some ((1/4)%Qp, to_agree (λ s: SAny.t, Some (to_agree (postS s)))) else ε) : threadsF) ≡ ◯ ((λ n: nat, if tid =? n then Some (1%Qp, to_agree (λ s: SAny.t, Some (to_agree (Q s)))) else ths_src_w n) : threadsF)).
         { f_equiv. intros y. rewrite !discrete_fun_lookup_op.
           destruct (decide (tid = y)).
@@ -750,10 +467,10 @@ Notation "E1 '------------------------------------------------------------------
       iAssert (Ist nths st_src st_tgt0) with "[THB THW COND]" as "IST".
       { iExists _, _, _, _. iFrame. iPureIntro. esplits; et. }
       w_force_l false. w_steps_l. w_force_l (tt). w_force_l (tt↑).
-      prep_l; iApply wpsim_full_guarantee_src_WP; iSplitL ""; et.
+      w_force_l; iSplitL ""; first done.
 
       w_call "IST".
-      w_step_l; prep_l; iApply wpsim_full_assume_src_WP; iIntros "[-> ->]".
+      w_steps_l. iDestruct "ASM" as  "[-> ->]".
       w_steps_l. hss; w_steps_l.
       w_steps_r. hss; w_steps_r.
       rewrite /cgetU.
@@ -793,10 +510,9 @@ Notation "E1 '------------------------------------------------------------------
 
   Theorem correct :
     ctx_refines
-      (SchA.t univ Spc_global Spc_user, SchA.InitCond)
+      (SchA.t υ n Spc_global Spc_user, SchA.InitCond)
       (SchI.t, emp%I).
   Proof.
     eapply main_adequacy. eapply sim; et.
   Qed.
-
 End SchIA. End SchIA.
