theories/lib/ltac2_lib.v
@@ -1,0 +1,102 @@
+(* NOTE : opening this file with VsCoq 2 will immediately crash the language server - use vscoq legacy instead *)
+From Ltac2 Require Import Ltac2.
+
+Ltac2 or t0 t1 :=
+  fun x =>
+    match! 'True with
+    | True => t0 x
+    | _ => t1 x
+    end.
+
+Ltac2 Type exn ::= [ TCSearchSuccess (constr) | TCSearchFail ].
+
+Ltac2 evar t n :=
+  let u := open_constr:(_: ltac:(exact_no_check $t)) in
+  match Constr.Unsafe.kind u with
+  | Constr.Unsafe.Cast v _ _ =>
+      Std.pose n u;
+      v
+  | _ => Control.throw Init.Assertion_failure
+  end
+.
+
+Ltac2 unshelve_evar e n :=
+  let v := evar e (Some n) in
+  match Constr.Unsafe.kind v with
+  | Constr.Unsafe.Evar e _ =>
+      Control.new_goal e
+  | _ => Control.throw Init.Assertion_failure
+  end
+.
+
+Ltac2 unshelve_evar1 e n :=
+  (ltac1:(e n|- unshelve evar (n: e))) (Ltac1.of_constr e) (Ltac1.of_ident n)
+.
+
+Ltac2 multiverse_execute tac :=
+  let l := Array.make 1 (None: constr option) in
+  Control.plus
+    (fun _ =>
+       let v := tac () in
+       Array.set l 0 (Some v);
+       Control.zero (Tactic_failure None)
+    )
+    (fun _ =>
+       match Array.get l 0 with
+       | Some c => c
+       | None => Control.zero (Tactic_failure None)
+       end).
+
+Ltac2 tcsearch e :=
+  multiverse_execute
+    (fun _ =>
+       let n := Fresh.in_goal ident:(_TC_) in
+       unshelve_evar e n > [|typeclasses_eauto];
+       Std.eval_unfold [(Std.VarRef n, Std.AllOccurrences)] (Control.hyp n)).
+
+Ltac2 tcsearch_alt e :=
+  Control.plus
+    (fun _ =>
+       let n := Fresh.in_goal ident:(_TC_) in
+       unshelve_evar e n > [|once typeclasses_eauto];
+       Control.zero (TCSearchSuccess (Std.eval_unfold [(Std.VarRef n, Std.AllOccurrences)] (Control.hyp n)))
+    )
+    (fun e =>
+       match e with
+       | TCSearchSuccess c => c
+       | _ => Control.zero e
+       end
+    )
+.
+
+Module TEST. Section TEST.
+  Variable A: Type.
+  Variable a b: A.
+
+  Class Foo (n: nat) := mk_Foo {}.
+  Global Instance foo: Foo 3 := mk_Foo _.
+
+  Class Bar (a: A) := mk_Bar { Bar_contents: A; }.
+
+  Instance bar: Bar a := mk_Bar _ b.
+
+  Goal True.
+    time (let _ := tcsearch_alt constr:(Foo 3) in ()).
+    time (let _ := tcsearch_alt constr:(Bar a) in ()).
+    time (do 100 (let _ := tcsearch constr:(Bar a) in ())).
+    exact I.
+  Qed.
+End TEST. End TEST.
+
+Ltac message :=
+  ltac2:(e |-
+           let e := Option.get (Ltac1.to_constr e) in
+           Message.print (Message.of_constr e))
+.
+
+Ltac tcsearch :=
+  ltac2:(e k |-
+           let e := Option.get (Ltac1.to_constr e) in
+           let v := tcsearch e in
+           Ltac1.apply k [Ltac1.of_constr v] Ltac1.run)
+.
