theories/simulations/wpsim/wpsim_tactics.v
@@ -1,0 +1,300 @@
+Require Import CRIS ltac2_lib.
+Require Export wpsim.
+
+From iris.proofmode Require Import coq_tactics environments.
+(* ● ◓ ○ *)
+Notation "E1 '------------------------------------------------------------------□' E2 '------------------------------------------------------------------∗' st_src st_tgt '------------------------------params------------------------------' ○ n E r g ps pt '-------------------------------wsim-------------------------------' itr_src itr_tgt" :=
+  (environments.envs_entails (Envs E1 E2 _) (wpsim _ _ _ _ None _ _ n E r g _ _ _ ps pt _ (st_src, itr_src) (st_tgt, itr_tgt)))
+    (at level 50, only printing,
+      format "E1 '------------------------------------------------------------------□' '//' E2 '------------------------------------------------------------------∗' '//' st_src '//' st_tgt '//' '------------------------------params------------------------------' '//' ○ '/' n '/' E '/' r '/' g '/' ps '/' pt '//' '-------------------------------wsim-------------------------------' '//' itr_src '//' '//' '//' itr_tgt '//'").
+Notation "E1 '------------------------------------------------------------------□' E2 '------------------------------------------------------------------∗' st_src st_tgt '------------------------------params------------------------------' ◓ n E r g ps pt '-------------------------------wsim-------------------------------' itr_src itr_tgt" :=
+  (environments.envs_entails (Envs E1 E2 _) (wpsim _ _ _ _ (Some false) _ _ n E r g _ _ _ ps pt _ (st_src, itr_src) (st_tgt, itr_tgt)))
+    (at level 50, only printing,
+      format "E1 '------------------------------------------------------------------□' '//' E2 '------------------------------------------------------------------∗' '//' st_src '//' st_tgt '//' '------------------------------params------------------------------' '//' ◓ '/' n '/' E '/' r '/' g '/' ps '/' pt '//' '-------------------------------wsim-------------------------------' '//' itr_src '//' '//' '//' itr_tgt '//'").
+Notation "E1 '------------------------------------------------------------------□' E2 '------------------------------------------------------------------∗' st_src st_tgt '------------------------------params------------------------------' ● n E r g ps pt '-------------------------------wsim-------------------------------' itr_src itr_tgt" :=
+  (environments.envs_entails (Envs E1 E2 _) (wpsim _ _ _ _ (Some true) _ _ n E r g _ _ _ ps pt _ (st_src, itr_src) (st_tgt, itr_tgt)))
+    (at level 50, only printing,
+      format "E1 '------------------------------------------------------------------□' '//' E2 '------------------------------------------------------------------∗' '//' st_src '//' st_tgt '//' '------------------------------params------------------------------' '//' ● '/' n '/' E '/' r '/' g '/' ps '/' pt '//' '-------------------------------wsim-------------------------------' '//' itr_src '//' '//' '//' itr_tgt '//'").
+Notation "E1 '------------------------------------------------------------------□' st_src st_tgt '------------------------------params------------------------------' ○ n E r g ps pt '-------------------------------wsim-------------------------------' itr_src itr_tgt" :=
+  (environments.envs_entails (Envs E1 Enil _) (wpsim _ _ _ _ None _ _ n E r g _ _ _ ps pt _ (st_src, itr_src) (st_tgt, itr_tgt)))
+    (at level 50, only printing,
+      format "E1 '------------------------------------------------------------------□' '//' st_src '//' st_tgt '//' '------------------------------params------------------------------' '//' ○ '/' n '/' E '/' r '/' g '/' ps '/' pt '//' '-------------------------------wsim-------------------------------' '//' itr_src '//' '//' '//' itr_tgt '//'").
+Notation "E1 '------------------------------------------------------------------□' st_src st_tgt '------------------------------params------------------------------' ◓ n E r g ps pt '-------------------------------wsim-------------------------------' itr_src itr_tgt" :=
+  (environments.envs_entails (Envs E1 Enil _) (wpsim _ _ _ _ (Some false) _ _ n E r g _ _ _ ps pt _ (st_src, itr_src) (st_tgt, itr_tgt)))
+    (at level 50, only printing,
+      format "E1 '------------------------------------------------------------------□' '//' st_src '//' st_tgt '//' '------------------------------params------------------------------' '//' ◓ '/' n '/' E '/' r '/' g '/' ps '/' pt '//' '-------------------------------wsim-------------------------------' '//' itr_src '//' '//' '//' itr_tgt '//'").
+Notation "E1 '------------------------------------------------------------------□' st_src st_tgt '------------------------------params------------------------------' ● n E r g ps pt '-------------------------------wsim-------------------------------' itr_src itr_tgt" :=
+  (environments.envs_entails (Envs E1 Enil _) (wpsim _ _ _ _ (Some true) _ _ n E r g _ _ _ ps pt _ (st_src, itr_src) (st_tgt, itr_tgt)))
+    (at level 50, only printing,
+      format "E1 '------------------------------------------------------------------□' '//' st_src '//' st_tgt '//' '------------------------------params------------------------------' '//' ● '/' n '/' E '/' r '/' g '/' ps '/' pt '//' '-------------------------------wsim-------------------------------' '//' itr_src '//' '//' '//' itr_tgt '//'").
+Notation "E2 '------------------------------------------------------------------∗' st_src st_tgt '------------------------------params------------------------------' ○ n E r g ps pt '-------------------------------wsim-------------------------------' itr_src itr_tgt" :=
+  (environments.envs_entails (Envs Enil E2 _) (wpsim _ _ _ _ None _ _ n E r g _ _ _ ps pt _ (st_src, itr_src) (st_tgt, itr_tgt)))
+    (at level 50, only printing,
+      format "E2 '------------------------------------------------------------------∗' '//' st_src '//' st_tgt '//' '------------------------------params------------------------------' '//' ○ '/' n '/' E '/' r '/' g '/' ps '/' pt '//' '-------------------------------wsim-------------------------------' '//' itr_src '//' '//' '//' itr_tgt '//'").
+Notation "E2 '------------------------------------------------------------------∗' st_src st_tgt '------------------------------params------------------------------' ◓ n E r g ps pt '-------------------------------wsim-------------------------------' itr_src itr_tgt" :=
+  (environments.envs_entails (Envs Enil E2 _) (wpsim _ _ _ _ (Some false) _ _ n E r g _ _ _ ps pt _ (st_src, itr_src) (st_tgt, itr_tgt)))
+    (at level 50, only printing,
+      format "E2 '------------------------------------------------------------------∗' '//' st_src '//' st_tgt '//' '------------------------------params------------------------------' '//' ◓ '/' n '/' E '/' r '/' g '/' ps '/' pt '//' '-------------------------------wsim-------------------------------' '//' itr_src '//' '//' '//' itr_tgt '//'").
+Notation "E2 '------------------------------------------------------------------∗' st_src st_tgt '------------------------------params------------------------------' ● n E r g ps pt '-------------------------------wsim-------------------------------' itr_src itr_tgt" :=
+  (environments.envs_entails (Envs Enil E2 _) (wpsim _ _ _ _ (Some true) _ _ n E r g _ _ _ ps pt _ (st_src, itr_src) (st_tgt, itr_tgt)))
+    (at level 50, only printing,
+      format "E2 '------------------------------------------------------------------∗' '//' st_src '//' st_tgt '//' '------------------------------params------------------------------' '//' ● '/' n '/' E '/' r '/' g '/' ps '/' pt '//' '-------------------------------wsim-------------------------------' '//' itr_src '//' '//' '//' itr_tgt '//'").
+
+(* additional *) 
+Notation "E1 '------------------------------------------------------------------□' E2 '------------------------------------------------------------------∗' st_src st_tgt '-------------------------------wsim-------------------------------' P '∗' 'WSIM'" :=
+  (environments.envs_entails (Envs E1 E2 _) (bi_sep P (wpsim _ _ _ _ _ _ _ _ _ _ _ _ _ _ _ _ _ (st_src, _) (st_tgt, _))))
+    (at level 50, only printing,
+      format "E1 '------------------------------------------------------------------□' '//' E2 '------------------------------------------------------------------∗' '//' st_src '//' st_tgt '//' '-------------------------------wsim-------------------------------' '//' P  '∗'  'WSIM' ").
+
+Notation "E1 '------------------------------------------------------------------□' E2 '------------------------------------------------------------------∗' st_src st_tgt '-------------------------------wsim-------------------------------' P '-∗' 'WSIM'" :=
+  (environments.envs_entails (Envs E1 E2 _) (bi_wand P (wpsim _ _ _ _ _ _ _ _ _ _ _ _ _ _ _ _ _ (st_src, _) (st_tgt, _))))
+    (at level 50, only printing,
+      format "E1 '------------------------------------------------------------------□' '//' E2 '------------------------------------------------------------------∗' '//' st_src '//' st_tgt '//' '-------------------------------wsim-------------------------------' '//' P  '-∗'  'WSIM' ").
+
+Ltac _w_step :=
+  match goal with
+  | [ |- environments.envs_entails _ (wpsim _ _ _ _ _ _ _ _ _ _ _ _ _ _ _ _ _ (_, Ret _) (_, Ret _))] =>
+      iApply wpsim_ret
+  | [ |- environments.envs_entails _ (wpsim _ _ _ _ _ _ _ _ _ _ _ _ _ _ _ _ _ (_, trigger (IO _ _) >>= _) (_, trigger (IO _ _) >>= _))] =>
+      iApply wpsim_io; iIntros "%"
+  | [ |- environments.envs_entails _ (wpsim _ _ _ _ _ _ _ _ _ _ _ _ _ _ _ _ _ (_, trigger (Spawn _ _) >>= _) (_, trigger (Spawn _ _) >>= _))] =>
+      iApply wpsim_spawn
+  end.
+
+Ltac _w_step_l :=
+  match goal with
+  | [ |- environments.envs_entails _ (wpsim _ _ _ _ _ _ _ _ _ _ _ _ _ _ _ _ _ (_, tau;; _) _) ] =>
+      iApply wpsim_tau_src
+  | [ |- environments.envs_entails _ (wpsim _ _ _ _ _ _ _ _ _ _ _ _ _ _ _ _ _ (_, Ret _ >>= _) _) ] =>
+      rewrite bind_ret_l
+  | [ |- environments.envs_entails _ (wpsim _ _ _ _ _ _ _ _ _ _ _ _ _ _ _ _ _ (_, trigger Tid >>= _) _) ] =>
+      iApply wpsim_tid_src
+  | [ |- environments.envs_entails _ (wpsim _ _ _ _ _ _ _ _ _ _ _ _ _ _ _ _ _ (_, trigger (Take _) >>= _) _) ] =>
+      let name := fresh "q" in iApply wpsim_take_src; iIntros (name)
+  | [ |- environments.envs_entails _ (wpsim _ _ _ _ _ ?υ _ ?n _ _ _ _ _ _ _ _ _ (_, trigger (Assume ?P) >>= _) _) ] =>
+      first [
+        tcsearch constr:(WP P υ n ⊤)
+          ltac:(fun c =>
+            iApply (wpsim_full_assume_src_WP _ _ _ _ _ _ _ _ _ _ _ _ _ _ _ _ _ _ _ (i:=c)); simpl);
+        match goal with
+        | [ |- environments.envs_entails _ (?P' -∗ _)] =>
+          unfold_precond_postcond P'; iIntrosFresh "ASM"
+        end
+      | unfold_precond_postcond P; iApply wpsim_assume_src; iIntrosFresh "ASM"
+      ]
+  | [ |- environments.envs_entails _ (wpsim _ _ _ _ _ _ _ _ _ _ _ _ _ _ _ _ _ (_, assume _ >>= _) _) ] =>
+      let name := fresh "asm" in iApply wpsim_asm_src; iIntros (name)
+  | [ |- environments.envs_entails _ (wpsim _ _ _ _ _ _ _ _ _ _ _ _ _ _ _ _ _ (_, (HMod.sandbox _ (trigger (SPut _ _))) >>= _) _) ] =>
+      iApply wpsim_sput_src_sandbox; [s;eauto|]
+  | [ |- environments.envs_entails _ (wpsim _ _ _ _ _ _ _ _ _ _ _ _ _ _ _ _ _ (_, (HMod.sandbox _ (trigger (SGet _))) >>= _) _) ] =>
+      iApply wpsim_sget_src_sandbox; [s;eauto|]
+  | [ |- environments.envs_entails _ (wpsim _ _ _ _ _ _ _ _ _ _ _ _ _ _ _ _ _ (_, unwrapU ?ox >>= _) _) ] =>
+      let name := fresh "q" in
+      iApply wpsim_unwrapU_src; iIntros (name) "%";
+      match goal with [ H: ?x = Some _ |- _ ] => let G := fresh "G" in rename H into G; try rewrite -> G in * end
+  end.
+
+Ltac _w_step_r :=
+  match goal with
+  (******* isim ******)
+  (** tgt **)
+  | [ |- environments.envs_entails _ (wpsim _ _ _ _ _ _ _ _ _ _ _ _ _ _ _ _ _ _ (_, tau;; _)) ] =>
+      iApply wpsim_tau_tgt
+  | [ |- environments.envs_entails _ (wpsim _ _ _ _ _ _ _ _ _ _ _ _ _ _ _ _ _ _ (_, Ret _ >>= _) ) ] =>
+      rewrite bind_ret_l
+  | [ |- environments.envs_entails _ (wpsim _ _ _ _ _ _ _ _ _ _ _ _ _ _ _ _ _ _ (_, trigger (Choose _) >>= _) ) ] =>
+      let name := fresh "q" in iApply wpsim_choose_tgt; iIntros (name)
+  | [ |- environments.envs_entails _ (wpsim _ _ _ _ _ _ _ _ _ _ _ _ _ _ _ _ _ _ (_, trigger (Guarantee ?P) >>= _) ) ] =>
+      unfold_precond_postcond P; iApply wpsim_guarantee_tgt; iIntrosFresh "GRT"
+  | [ |- environments.envs_entails _ (wpsim _ _ _ _ _ _ _ _ _ _ _ _ _ _ _ _ _ _ (_, guarantee _ >>= _)) ] =>
+      let name := fresh "grt" in iApply wpsim_guar_tgt; iIntros (name)
+  | [ |- environments.envs_entails _ (wpsim _ _ _ _ _ _ _ _ _ _ _ _ _ _ _ _ _ _ (_, (HMod.sandbox _ (trigger (SPut _ _))) >>= _)) ] =>
+      iApply wpsim_sput_tgt_sandbox; [s; eauto|]
+  | [ |- environments.envs_entails _ (wpsim _ _ _ _ _ _ _ _ _ _ _ _ _ _ _ _ _ _ (_, (HMod.sandbox _ (trigger (SGet _))) >>= _)) ] =>
+      iApply wpsim_sget_tgt_sandbox; [s; eauto|]
+  (* 
+  | [ |- environments.envs_entails _ (isim _ _ _ _ _ _ _ _ _ _ _ _ (_, unwrapN ?ox >>= _)) ] =>
+      let name := fresh "q" in
+      iApply isim_unwrapN_tgt; iIntros (name) "%";
+      match goal with [ H: ?x = Some _ |- _ ] => let G := fresh "G" in rename H into G; try rewrite -> G in * end
+*)
+  | [ |- environments.envs_entails _ (wpsim _ _ _ _ _ _ _ _ _ _ _ _ _ _ _ _ _ _ (_, trigger Tid >>= _)) ] =>
+      iApply wpsim_tid_tgt
+  end.
+
+Ltac w_step_l_core :=
+  _w_step_l; try alist_find_simpl; s; des_pairs; s.
+Ltac w_step_r_core :=
+  _w_step_r; try alist_find_simpl; s; des_pairs; s.
+
+Ltac _w_force_l :=
+  match goal with
+  | [ |- environments.envs_entails _ (wpsim _ _ _ _ _ _ _ _ _ _ _ _ _ _ _ _ _ (_, trigger (Choose ?T) >>= _) _) ] =>
+      iApply wpsim_choose_src
+  | [ |- environments.envs_entails _ (wpsim _ _ _ _ _ ?υ _ ?n _ _ _ _ _ _ _ _ _ (_, trigger (Guarantee ?P) >>= _) _) ] =>
+      first [
+        tcsearch constr:(WP P υ n ⊤)
+          ltac:(fun c =>
+            iApply (wpsim_full_guarantee_src_WP _ _ _ _ _ _ _ _ _ _ _ _ _ _ _ _ _ _ _ (i:=c)); simpl);
+        match goal with
+        | [ |- environments.envs_entails _ (?P' ∗ _)] =>
+          unfold_precond_postcond P'
+        end
+      | unfold_precond_postcond P; iApply wpsim_guarantee_src
+      ]
+  | [ |- environments.envs_entails _ (wpsim _ _ _ _ _ _ _ _ _ _ _ _ _ _ _ _ _ (_, unwrapN _ >>= _) _) ] =>
+      iApply wpsim_unwrapN_src
+  (* | [ |- environments.envs_entails _ (isim _ _ _ _ _ _ _ _ _ _ _ (_, guarantee _ >>= _) _) ] =>
+      iApply isim_guar_src *)
+  end.
+
+(* Ltac preprocess_l tac :=
+  let marker := fresh "MARKER" in
+  set_marker marker;
+  hide_ihyps;
+  hide_itree_r;
+  prep;
+  tac;
+  show_until marker.
+
+Ltac preprocess_r tac :=
+  let marker := fresh "MARKER" in
+  set_marker marker;
+  hide_ihyps;
+  hide_itree_l;
+  prep;
+  tac;
+  show_until marker.
+
+Ltac preprocess_both tac :=
+  let marker := fresh "MARKER" in
+  set_marker marker;
+  hide_ihyps;
+  hide_itree_l; prep; show_itree;
+  hide_itree_r; prep; show_itree;
+  tac;
+  show_until marker.
+   *)
+Ltac w_force_l_core :=
+  let marker := fresh "MARKER" in
+  set_marker marker;
+  hide_ihyps;
+  hide_itree_r;
+  prep;
+  _w_force_l;
+  show_until marker.
+
+Tactic Notation "w_force_l" :=
+  w_force_l_core; try (iExists _).
+
+Tactic Notation "w_force_l" uconstr(p) :=
+  w_force_l_core; iExists p.
+
+Ltac w_step :=
+  let marker := fresh "MARKER" in
+  set_marker marker;
+  hide_ihyps;
+  hide_itree_r; prep; show_itree;
+  hide_itree_l; prep; show_itree;
+  _w_step;
+  show_until marker.
+
+Ltac w_step_l :=
+  let marker := fresh "MARKER" in
+  set_marker marker;
+  hide_ihyps;
+  hide_itree_r;
+  prep;
+  w_step_l_core;
+  show_until marker.
+
+Ltac w_steps_l :=
+  let marker := fresh "MARKER" in
+  set_marker marker;
+  hide_ihyps;
+  hide_itree_r;
+  (hrepeat do 1 (prep; w_step_l_core));
+  show_until marker.
+
+Ltac w_step_r :=
+  let marker := fresh "MARKER" in
+  set_marker marker;
+  hide_ihyps;
+  hide_itree_l;
+  prep;
+  w_step_r_core;
+  show_until marker.
+
+Ltac w_steps_r :=
+  let marker := fresh "MARKER" in
+  set_marker marker;
+  hide_ihyps;
+  hide_itree_l;
+  (hrepeat do 1 (prep; w_step_r_core));
+  show_until marker.
+
+Ltac by_coind CIH :=
+  iApply wpsim_progress; iApply wpsim_base;
+  iSpecialize (CIH $! _);
+  (hrepeat do 1 first[instantiate (1:= (_,_))|instantiate (1:= existT _ _)]); s; grind;
+  iApply CIH.
+
+Ltac w_call hyps :=
+  let marker := fresh "MARKER" in
+  set_marker marker;
+  hide_ihyps;
+  hide_itree_r; prep; show_itree;
+  hide_itree_l; prep; show_itree;
+  iApply wpsim_call;
+  show_until marker;
+  iSplitL hyps; [try done | iIntros "% % % % % %"; iIntrosFresh "IST"];
+  move_aux.
+
+Ltac yield hyps :=
+  let marker := fresh "MARKER" in
+  set_marker marker;
+  hide_ihyps;
+  hide_itree_r; prep; show_itree;
+  hide_itree_l; prep; show_itree;
+  iApply wpsim_yield
+  ; show_until marker
+  ; iSplitL hyps; [try done | iIntros "% % % % %"; iIntrosFresh "IST"]
+  ; move_aux
+  .
+
+Ltac init_simF :=
+  pre_simF;
+  alist_find_simpl;
+  let H := fresh "H" in intro H; inv H;
+  alist_find_simpl;
+  post_simF;
+  step_l.
+
+Ltac init_wpsim :=
+  init_simF;
+  prep_l;
+  match goal with
+  | [ |- environments.envs_entails _ (isim _ _ _ _ _ _ _ _ _ _ _ (_, trigger (Take _) >>= _) _)] =>
+    let name := fresh "q" in let n := fresh "n" in iApply isim_take_src; iIntros (name);
+      prep; let varg := fresh "varg" in iApply isim_take_src; iIntros (varg);
+      prep;
+      match goal with
+      | [ |- environments.envs_entails _ (isim _ _ _ _ _ _ _ _ _ _ _  (_, trigger (Assume ?P) >>= _) _) ] =>
+        unfold_precond_postcond P; iApply isim_Assume_src; iIntros "[I ASM]";
+        iApply wpsim_init; iSplitR "I"; last iExact "I"
+      end
+  end.
+
+Ltac unfold_iter_l :=
+  let marker := fresh "MARKER" in
+  set_marker marker;
+  hide_ihyps;
+  hide_itree_r; rewrite unfold_iter_eq; show_itree;
+  show_until marker.
+
+Ltac unfold_iter_r :=
+  let marker := fresh "MARKER" in
+  set_marker marker;
+  hide_ihyps;
+  hide_itree_l; rewrite unfold_iter_eq; show_itree;
+  show_until marker.
